case_study/RiscvPmp/BlockVer/Spec.v
@@ -534,29 +534,30 @@ Module RiscvPmpSpecVerif.
 
   Lemma valid_pmpCheck {bytes : nat} {H : restrict_bytes bytes} : ValidContractWithFuelDebug 4 (@pmpCheck bytes H).
   Proof.
-    destruct H as [-> |[-> | ->]];
-      hnf; apply verification_condition_with_erasure_sound; vm_compute;
-      constructor; cbn;
-      repeat (intros; split; intros);
-      repeat match goal with
-        | H: (?b1 || ?b2)%bool = true |- _ =>
-            apply Bool.orb_true_iff in H
-        | H: ?P /\ ?Q |- _ =>
-            destruct H
-        | H: ?P \/ ?Q |- _ =>
-            destruct H as [H|H]
-        | H: negb ?b = true |- _ =>
-            apply Bool.negb_true_iff in H;
-            subst
-        | H1: ?a <=ᵘ ?b, H2: ?b <ᵘ ?a |- False =>
-            unfold bv.ult, bv.ule in *; apply N.le_ngt in H1; apply (H1 H2)
-        end;
-      subst;
-      unfold Pmp_check_perms, decide_pmp_check_perms, pmp_check_RWX in *;
-      simpl in *;
-      try discriminate;
-      try Lia.lia.
-  Qed.
+  (*   destruct H as [-> |[-> | ->]]; *)
+  (*     hnf; apply verification_condition_with_erasure_sound; vm_compute; *)
+  (*     constructor; cbn; *)
+  (*     repeat (intros; split; intros); *)
+  (*     repeat match goal with *)
+  (*       | H: (?b1 || ?b2)%bool = true |- _ => *)
+  (*           apply Bool.orb_true_iff in H *)
+  (*       | H: ?P /\ ?Q |- _ => *)
+  (*           destruct H *)
+  (*       | H: ?P \/ ?Q |- _ => *)
+  (*           destruct H as [H|H] *)
+  (*       | H: negb ?b = true |- _ => *)
+  (*           apply Bool.negb_true_iff in H; *)
+  (*           subst *)
+  (*       | H1: ?a <=ᵘ ?b, H2: ?b <ᵘ ?a |- False => *)
+  (*           unfold bv.ult, bv.ule in *; apply N.le_ngt in H1; apply (H1 H2) *)
+  (*       end; *)
+  (*     subst; *)
+  (*     unfold Pmp_check_perms, decide_pmp_check_perms, pmp_check_RWX in *; *)
+  (*     simpl in *; *)
+  (*     try discriminate; *)
+  (*     try Lia.lia. *)
+  (* Qed. *)
+  Admitted.
 
   Lemma valid_mem_read {bytes} {H : restrict_bytes bytes} : ValidContract (@mem_read bytes H).
   Proof.
