case_study/RiscvPmp/FemtoKernel.v
@@ -112,6 +112,7 @@ Import BlockVerificationDerived2.
       fun mt => match mt with
                 | OFF => bv.zero
                 | TOR => bv.one
+                | NA4 => bv.of_nat 2
                 end.
 
     Definition pure_pmpcfg_ent_to_bits : Pmpcfg_ent -> Val (ty.bvec byte) :=
